src/program_logic/recovery_adequacy.v
@@ -14,41 +14,41 @@ Implicit Types s : stuckness.
 Implicit Types k : nat.
 Implicit Types P : iProp Σ.
 Implicit Types Φ : val Λ → iProp Σ.
-Implicit Types Φinv : invG Σ → crashG Σ → pbundleG T Σ → iProp Σ.
-Implicit Types Φc : invG Σ → crashG Σ → pbundleG T Σ → val Λ → iProp Σ.
+Implicit Types Φinv : crashG Σ → pbundleG T Σ → iProp Σ.
+Implicit Types Φc : crashG Σ → pbundleG T Σ → val Λ → iProp Σ.
 Implicit Types v : val Λ.
 Implicit Types e : expr Λ.
 
 Notation wptp s k t := ([∗ list] ef ∈ t, WPC ef @ s; k; ⊤ {{ fork_post }} {{ True }})%I.
 
-Fixpoint step_fupdN_fresh (ns: list nat) Hi0 (Hc0: crashG Σ) t0
-         (P: invG Σ → crashG Σ → pbundleG T Σ → iProp Σ) {struct ns} :=
+Fixpoint step_fupdN_fresh (ns: list nat) (Hc0: crashG Σ) t0
+         (P: crashG Σ → pbundleG T Σ → iProp Σ) {struct ns} :=
   match ns with
-  | [] => P Hi0 Hc0 t0
+  | [] => P Hc0 t0
   | (n :: ns) =>
-    (|={⊤}[∅]▷=>^(S (S n)) |={⊤, ∅}_2=>
-     ∀ Hi' Hc', NC 1 ={⊤}=∗ (∃ t' : pbundleG T Σ, step_fupdN_fresh ns Hi' Hc' t' P))%I
+    (|={⊤}[∅]▷=>^(S (S n)) |={⊤, ⊤}_2=>
+     ∀ Hc', NC 1 ={⊤}=∗ (∃ t' : pbundleG T Σ, step_fupdN_fresh ns Hc' t' P))%I
   end.
 
-Lemma step_fupdN_fresh_snoc (ns: list nat) n Hi0 Hc0 t0 Q:
-  step_fupdN_fresh (ns ++ [n]) Hi0 Hc0 t0 Q ≡
-  step_fupdN_fresh (ns) Hi0 Hc0 t0
-    (λ Hi Hc' _, |={⊤}[∅]▷=>^(S (S n)) |={⊤, ∅}_2=> ∀ Hi' Hc', NC 1={⊤}=∗ ∃ t', Q Hi' Hc' t')%I.
+Lemma step_fupdN_fresh_snoc (ns: list nat) n Hc0 t0 Q:
+  step_fupdN_fresh (ns ++ [n]) Hc0 t0 Q ≡
+  step_fupdN_fresh (ns) Hc0 t0
+    (λ Hc' _, |={⊤}[∅]▷=>^(S (S n)) |={⊤, ⊤}_2=> ∀ Hc', NC 1={⊤}=∗ ∃ t', Q Hc' t')%I.
 Proof.
   apply (anti_symm (⊢)%I).
-  - revert Hi0 Hc0 t0 Q.
-    induction ns => ????; first by auto.
+  - revert Hc0 t0 Q.
+    induction ns => ???; first by auto.
     iIntros "H".
     iApply (step_fupdN_wand ⊤ ∅ with "[H] []"); auto.
     iIntros "H".
     iMod "H". iModIntro. iMod "H". iModIntro. iNext.
     iMod "H". iModIntro. iMod "H". iModIntro. iNext.
     iMod "H". iModIntro. iMod "H". iModIntro.
-    iIntros (??) "HNC".
-    iMod ("H" $! _ _ with "[$]") as (?) "H".
+    iIntros (?) "HNC".
+    iMod ("H" $! _ with "[$]") as (?) "H".
     iExists _. by iApply IHns.
-  - revert Hi0 Hc0 t0 Q.
-    induction ns => ???? //=.
+  - revert Hc0 t0 Q.
+    induction ns => ??? //=.
     do 3 f_equiv.
     iIntros "H".
     iApply (step_fupdN_wand with "H"); auto.
@@ -59,14 +59,14 @@ Proof.
     iMod "H". do 2 iModIntro.
     iMod "H". iModIntro.
     iMod "H". iModIntro.
-    iIntros (??) "HNC".
-    iMod ("H" $! _ _ with "[$]") as (?) "H".
+    iIntros (?) "HNC".
+    iMod ("H" $! _ with "[$]") as (?) "H".
     iExists _. by iApply IHns.
 Qed.
 
-Lemma step_fupdN_fresh_pattern_wand {H: invG Σ} n (Q Q': iProp Σ):
-  (|={⊤}[∅]▷=>^n |={⊤, ∅}_2=> Q) -∗ (Q -∗ Q') -∗
-  (|={⊤}[∅]▷=>^n |={⊤, ∅}_2=> Q').
+Lemma step_fupdN_fresh_pattern_fupd {H: invG Σ} n (Q Q': iProp Σ):
+  (|={⊤}[∅]▷=>^n |={⊤, ⊤}_2=> Q) -∗ (Q ={⊤}=∗ Q') -∗
+  (|={⊤}[∅]▷=>^n |={⊤, ⊤}_2=> Q').
 Proof.
   iIntros "H Hwand". simpl.
   iApply (step_fupdN_wand with "H").
@@ -75,8 +75,23 @@ Proof.
   iMod "H". iModIntro.
   iMod "H". do 2 iModIntro.
   iMod "H". iModIntro.
-  iMod "H". iModIntro.
-  by iApply "Hwand".
+  iMod "H". by iMod ("Hwand" with "[$]").
+Qed.
+
+Lemma step_fupdN_fresh_pattern_bupd {H: invG Σ} n (Q Q': iProp Σ):
+  (|={⊤}[∅]▷=>^n |={⊤, ⊤}_2=> Q) -∗ (Q ==∗ Q') -∗
+  (|={⊤}[∅]▷=>^n |={⊤, ⊤}_2=> Q').
+Proof.
+  iIntros "H Hwand". iApply (step_fupdN_fresh_pattern_fupd with "H").
+  iIntros. by iMod ("Hwand" with "[$]").
+Qed.
+
+Lemma step_fupdN_fresh_pattern_wand {H: invG Σ} n (Q Q': iProp Σ):
+  (|={⊤}[∅]▷=>^n |={⊤, ⊤}_2=> Q) -∗ (Q -∗ Q') -∗
+  (|={⊤}[∅]▷=>^n |={⊤, ⊤}_2=> Q').
+Proof.
+  iIntros "H Hwand". iApply (step_fupdN_fresh_pattern_bupd with "H").
+  iIntros. by iApply "Hwand".
 Qed.
 
 Lemma step_fupdN_fresh_pattern_plain {H: invG Σ} n (Q: iProp Σ) `{!Plain Q}:
@@ -106,17 +121,30 @@ Proof.
   iMod "H". eauto.
 Qed.
 
-Lemma step_fupdN_fresh_wand (ns: list nat) Hi0 Hc0 t0 Q Q':
-  step_fupdN_fresh (ns) Hi0 Hc0 t0 Q -∗ (∀ Hinv Hc t, Q Hinv Hc t -∗ Q' Hinv Hc t)
-  -∗ step_fupdN_fresh ns Hi0 Hc0 t0 Q'.
+Lemma step_fupdN_fresh_pattern_plain'' {H: invG Σ} n (Q: iProp Σ) `{!Plain Q}:
+  (|={⊤}[∅]▷=>^(S n) |={⊤, ⊤}_2=> Q) -∗
+  (|={⊤}=> ▷^(S (S (S (S n)))) Q).
 Proof.
-  revert Hi0 Hc0 t0.
-  induction ns => ???.
+  iIntros "H".
+  iDestruct (step_fupdN_wand with "H []") as "H".
+  { iApply step_fupdN_inner_plain'. }
+  rewrite -step_fupdN_S_fupd.
+  iMod (step_fupdN_plain with "H") as "H".
+  iModIntro. iNext. rewrite -?later_laterN ?laterN_later. iNext.
+  iMod "H". eauto.
+Qed.
+
+Lemma step_fupdN_fresh_wand (ns: list nat) Hc0 t0 Q Q':
+  step_fupdN_fresh (ns) Hc0 t0 Q -∗ (∀ Hc t, Q Hc t -∗ Q' Hc t)
+  -∗ step_fupdN_fresh ns Hc0 t0 Q'.
+Proof.
+  revert Hc0 t0.
+  induction ns => ??.
   - iIntros "H Hwand". iApply "Hwand". eauto.
   - iIntros "H Hwand". rewrite /step_fupdN_fresh -/step_fupdN_fresh.
     iApply (step_fupdN_fresh_pattern_wand with "H [Hwand]").
     iIntros "H". (* iMod "H". iModIntro. *)
-    iIntros (Hi' Hc') "HNC". iSpecialize ("H" $! Hi' Hc' with "[$]"). iMod "H" as (?) "H".
+    iIntros (Hc') "HNC". iSpecialize ("H" $! Hc' with "[$]"). iMod "H" as (?) "H".
     iExists _. iApply (IHns with "H"). eauto.
 Qed.
 
@@ -126,55 +154,6 @@ Fixpoint fresh_later_count (ns: list nat) :=
   | n :: ns' => (S (S (S (S (S n))))) + fresh_later_count ns'
   end.
 
-Lemma step_fupdN_fresh_plain `{!invPreG Σ} `{!crashPreG Σ} P `{!Plain P} ns n:
-  (∀ Hinv' Hc', NC 1-∗ |={⊤}=> ∃ t, step_fupdN_fresh ns Hinv' Hc' t
-                  (λ _ _ _, |={⊤}[∅]▷=>^(S n) |={⊤, ∅}_2=> P)) -∗
-  ▷^(fresh_later_count ns + S n) P.
-Proof.
-  iIntros "H".
-  iInduction ns as [| n' ns] "IH".
-  - rewrite /step_fupdN_fresh.
-    iApply (bupd_plain (▷^(_) P)%I); try (iPureIntro; apply _).
-    iMod wsat_alloc' as (Hinv) "(Hw&HE)".
-    iMod NC_alloc as (Hc) "HNC".
-    iSpecialize ("H" $! Hinv Hc with "HNC").
-    rewrite {1}uPred_fupd_eq {1}/uPred_fupd_def.
-    iDestruct (ownE_weaken _ (AlwaysEn ∪ MaybeEn ⊤) with "HE") as "HE"; first by set_solver.
-    iMod ("H" with "[$]") as "[>Hw [>HE >H]]".
-    iDestruct ("H") as (_) "H".
-    iDestruct (step_fupdN_fresh_pattern_plain' _ (P)%I with "H") as "H".
-    rewrite {1}uPred_fupd_eq {1}/uPred_fupd_def.
-    iMod ("H" with "[$]") as "[Hw [HE >?]]"; eauto.
-  - iMod wsat_alloc' as (Hinv) "(Hw&HE)".
-    iMod NC_alloc as (Hc) "HNC".
-    iSpecialize ("H" $! Hinv).
-    rewrite {1}uPred_fupd_eq {1}/uPred_fupd_def.
-    iDestruct (ownE_weaken _ (AlwaysEn ∪ MaybeEn ⊤) with "HE") as "HE"; first by set_solver.
-    iMod ("H" with "HNC [$]") as "[>Hw [>HE >H]]".
-    iDestruct "H" as (t) "H".
-    rewrite /step_fupdN_fresh -/step_fupdN_fresh.
-    iDestruct (step_fupdN_fresh_pattern_wand _ _
-                  (▷^(fresh_later_count ns + _) P)%I
-                 with "H [IH]") as "H".
-    { iIntros "H". iApply "IH". iIntros. iMod ("H" with "[$]"). iModIntro. eauto. }
-    iDestruct (step_fupdN_fresh_pattern_plain' with "H") as "H".
-    rewrite {1}uPred_fupd_eq {1}/uPred_fupd_def.
-    iMod ("H" with "[$]") as "[Hw [HE >H]]".
-    simpl. rewrite ?laterN_plus. iApply "H".
-Qed.
-
-(* XXX this probably needs to be tweaked. *)
-Lemma step_fupdN_fresh_soundness `{!invPreG Σ} `{!crashPreG Σ} (φ : Prop) ns n:
-  (∀ (Hinv : invG Σ) (Hc: crashG Σ), NC 1-∗ (|={⊤}=> (∃ t0, step_fupdN_fresh ns Hinv Hc t0
-                             (λ _ _ _, |={⊤}[∅]▷=>^((S (S n))) |={⊤, ∅}_2=> ⌜φ⌝)))%I) →
-  φ.
-Proof.
-  intros Hiter.
-  eapply (soundness (M:=iResUR Σ) _  (fresh_later_count ns + _)); simpl.
-  rewrite laterN_plus.
-  iApply step_fupdN_fresh_plain. iIntros (Hinv Hc). iApply Hiter.
-Qed.
-
 (*
 Notation "|={ E }=>_( t ) Q" := (fupd (FUpd := t) E E Q)
  (at level 99) : bi_scope.
@@ -182,12 +161,12 @@ Notation "P ={ E }=∗_ t Q" := (P -∗ |={E}=>_(t) Q)%I
  (at level 99) : bi_scope.
 *)
 
-Lemma wptp_recv_strong_normal_adequacy Φ Φinv Φr κs' s k Hi Hc t n ns r1 e1 t1 κs t2 σ1 σ2 :
+Lemma wptp_recv_strong_normal_adequacy Φ Φinv Φr κs' s k Hc t n ns r1 e1 t1 κs t2 σ1 σ2 :
   nrsteps (CS := CS) r1 (ns ++ [n]) (e1 :: t1, σ1) κs (t2, σ2) Normal →
   state_interp σ1 (κs ++ κs') (length t1) -∗
-  wpr s k Hi Hc t ⊤ e1 r1 Φ Φinv Φr -∗
-  wptp s k t1 -∗ NC 1-∗ step_fupdN_fresh ns Hi Hc t (λ Hi' Hc' t',
-    ⌜ Hi' = Hi ∧ Hc' = Hc ∧ t' = t ⌝ ∗
+  wpr s k Hc t ⊤ e1 r1 Φ Φinv Φr -∗
+  wptp s k t1 -∗ NC 1-∗ step_fupdN_fresh ns Hc t (λ Hc' t',
+    ⌜ Hc' = Hc ∧ t' = t ⌝ ∗
     (|={⊤}[∅]▷=>^(S n) ∃ e2 t2',
     ⌜ t2 = e2 :: t2' ⌝ ∗
     ⌜ ∀ e2, s = NotStuck → e2 ∈ t2 → (is_Some (to_val e2) ∨ reducible e2 σ2) ⌝ ∗
@@ -207,28 +186,27 @@ Proof.
     first by (eapply nrsteps_normal_empty_prefix; eauto).
   inversion H. subst.
   rewrite /step_fupdN_fresh.
-  rewrite perennial_invG.
   iSplitL ""; first by eauto.
   iApply (step_fupdN_wand with "H"); auto.
 Qed.
 
-Lemma wptp_recv_strong_crash_adequacy Φ Φinv Φinv' Φr κs' s k Hi Hc t ns n r1 e1 t1 κs t2 σ1 σ2 :
+Lemma wptp_recv_strong_crash_adequacy Φ Φinv Φinv' Φr κs' s k Hc t ns n r1 e1 t1 κs t2 σ1 σ2 :
   nrsteps (CS := CS) r1 (ns ++ [n]) (e1 :: t1, σ1) κs (t2, σ2) Crashed →
   state_interp σ1 (κs ++ κs') (length t1) -∗
-  wpr s k Hi Hc t ⊤ e1 r1 Φ Φinv Φr -∗
-  □ (∀ Hi' Hc' t', Φinv Hi' Hc' t' -∗ □ Φinv' Hi' Hc' t') -∗
-  wptp s k t1 -∗ NC 1-∗ step_fupdN_fresh ns Hi Hc t (λ Hi' Hc' t',
+  wpr s k Hc t ⊤ e1 r1 Φ Φinv Φr -∗
+  □ (∀ Hc' t', Φinv Hc' t' -∗ □ Φinv' Hc' t') -∗
+  wptp s k t1 -∗ NC 1-∗ step_fupdN_fresh ns Hc t (λ Hc' t',
     (|={⊤}[∅]▷=>^(S (S n)) ∃ e2 t2',
     ⌜ t2 = e2 :: t2' ⌝ ∗
     ⌜ ∀ e2, s = NotStuck → e2 ∈ t2 → (is_Some (to_val e2) ∨ reducible e2 σ2) ⌝ ∗
     state_interp σ2 κs' (length t2') ∗
-    from_option (Φr Hi' Hc' t') True (to_val e2) ∗
-    □ Φinv' Hi' Hc' t' ∗
+    from_option (Φr Hc' t') True (to_val e2) ∗
+    □ Φinv' Hc' t' ∗
     ([∗ list] v ∈ omap to_val t2', fork_post v) ∗
     NC 1)).
 Proof.
-  revert Hi Hc t e1 t1 κs κs' t2 σ1 σ2 Φ.
-  induction ns as [|n' ns' IH] => Hi Hc t e1 t1 κs κs' t2 σ1 σ2 Φ.
+  revert Hc t e1 t1 κs κs' t2 σ1 σ2 Φ.
+  induction ns as [|n' ns' IH] => Hc t e1 t1 κs κs' t2 σ1 σ2 Φ.
   { rewrite app_nil_l.
     inversion 1.
     match goal with
@@ -243,23 +221,28 @@ Proof.
   rewrite Nat_iter_S.
   iApply (step_fupdN_later _ _ 1); first by set_solver+. iNext.
   iPoseProof (@wptp_strong_crash_adequacy with "[$] [$] [$]") as "H"; eauto.
-  rewrite perennial_crashG perennial_invG.
+  rewrite perennial_crashG.
   iSpecialize ("H" with "[$]").
   iApply (step_fupdN_wand _ _ (S n') with "H").
   iIntros "H".
-  iMod "H". iModIntro. iModIntro. iNext.
+  iMod "H".
+  iMod (fupd_intro_mask' _ ∅) as "Hclo"; first set_solver. do 2 iModIntro. iNext.
   iDestruct "H" as (e2 t2' ?) "(H&Hσ&HC)".
-  iMod ("H" with "[//] Hσ") as "H". iModIntro.
-  iModIntro. iNext. do 2 iModIntro.
+  iMod ("Hclo") as "_".
+  iMod ("H" with "[//] Hσ") as "H".
+  iMod (fupd_intro_mask' _ ∅) as "Hclo"; first set_solver. do 2 iModIntro. iNext.
+  iModIntro.
+  iMod ("Hclo") as "_".
+  iModIntro.
   destruct s0.
-  - iIntros (Hi' Hc') "HNC". iSpecialize ("H" $! Hi' Hc' with "[$]").
+  - iIntros (Hc') "HNC". iSpecialize ("H" $! Hc' with "[$]").
     iMod "H" as (t') "(Hσ&Hr&HNC)".
     iDestruct "Hr" as "(_&Hr)".
     iPoseProof (IH with "[Hσ] Hr [] [] HNC") as "H"; eauto.
-  - iIntros (Hi' Hc') "HNC".
-    iMod ("H" $! Hi' Hc' with "[$]") as (t') "(Hσ&Hr&HNC)".
+  - iIntros (Hc') "HNC".
+    iMod ("H" $! Hc' with "[$]") as (t') "(Hσ&Hr&HNC)".
     iExists t'.
-    iAssert (□Φinv' Hi' Hc' t')%I as "#Hinv'".
+    iAssert (□Φinv' Hc' t')%I as "#Hinv'".
     { iDestruct "Hr" as "(Hr&_)".
       iApply "Hinv". eauto.
     }
@@ -267,26 +250,26 @@ Proof.
     iDestruct (wptp_recv_strong_normal_adequacy with "[Hσ] [Hr] [] HNC") as "H"; eauto.
     iApply (step_fupdN_fresh_wand with "H").
     iModIntro.
-    iIntros (???) "H".
-    iDestruct "H" as ((?&?&?)) "H". subst.
+    iIntros (??) "H".
+    iDestruct "H" as ((?&?)) "H". subst.
     iClear "HC".
     iApply (step_fupdN_wand with "H"); auto.
     iFrame "Hinv'". iApply step_fupd_intro; first by set_solver. iNext. eauto.
 Qed.
 
-Lemma wptp_recv_strong_adequacy Φ Φinv Φinv' Φr κs' s k Hi Hc t ns n r1 e1 t1 κs t2 σ1 σ2 stat :
+Lemma wptp_recv_strong_adequacy Φ Φinv Φinv' Φr κs' s k Hc t ns n r1 e1 t1 κs t2 σ1 σ2 stat :
   nrsteps (CS := CS) r1 (ns ++ [n]) (e1 :: t1, σ1) κs (t2, σ2) stat →
   state_interp σ1 (κs ++ κs') (length t1) -∗
-  wpr s k Hi Hc t ⊤ e1 r1 Φ Φinv Φr -∗
-  □ (∀ Hi' Hc' t', Φinv Hi' Hc' t' -∗ □ Φinv' Hi' Hc' t') -∗
-  wptp s k t1 -∗ NC 1-∗ step_fupdN_fresh ns Hi Hc t (λ Hi' Hc' t',
+  wpr s k Hc t ⊤ e1 r1 Φ Φinv Φr -∗
+  □ (∀ Hc' t', Φinv Hc' t' -∗ □ Φinv' Hc' t') -∗
+  wptp s k t1 -∗ NC 1-∗ step_fupdN_fresh ns Hc t (λ Hc' t',
     (|={⊤}[∅]▷=>^(S (S n)) ∃ e2 t2',
     ⌜ t2 = e2 :: t2' ⌝ ∗
     ⌜ ∀ e2, s = NotStuck → e2 ∈ t2 → (is_Some (to_val e2) ∨ reducible e2 σ2) ⌝ ∗
     state_interp σ2 κs' (length t2') ∗
     (match stat with
-     | Normal => ⌜ Hi' = Hi ∧ Hc' = Hc ∧ t' = t ⌝ ∗ from_option Φ True (to_val e2)
-     | Crashed => from_option (Φr Hi' Hc' t') True (to_val e2) ∗ □ Φinv' Hi' Hc' t'
+     | Normal => ⌜ Hc' = Hc ∧ t' = t ⌝ ∗ from_option Φ True (to_val e2)
+     | Crashed => from_option (Φr Hc' t') True (to_val e2) ∗ □ Φinv' Hc' t'
      end)  ∗
     ([∗ list] v ∈ omap to_val t2', fork_post v) ∗
     NC 1)).
@@ -294,15 +277,15 @@ Proof.
   intros. destruct stat.
   - iIntros. iDestruct (wptp_recv_strong_crash_adequacy with "[$] [$] [$] [$] [$]") as "H"; eauto.
     iApply (step_fupdN_fresh_wand with "H").
-    iIntros (???) "H".
+    iIntros (??) "H".
     iApply (step_fupdN_wand with "H"); auto.
     iIntros "H".
     iDestruct "H" as (????) "(H&?&?&?)". iExists _, _.
     repeat (iSplitL ""; try iFrame; eauto).
   - iIntros. iDestruct (wptp_recv_strong_normal_adequacy with "[$] [$] [$] [$]") as "H"; eauto.
     iApply (step_fupdN_fresh_wand with "H").
-    iIntros (???) "H".
-    iDestruct "H" as ((?&?&?)) "H". subst.
+    iIntros (??) "H".
+    iDestruct "H" as ((?&?)) "H". subst.
     iApply (step_fupdN_wand with "H"); auto.
     iApply step_fupd_intro; first by set_solver. iNext.
     iIntros "H".
@@ -311,6 +294,65 @@ Proof.
 Qed.
 
 End recovery_adequacy.
+
+Lemma step_fupdN_fresh_plain {Λ CS T Σ} `{!invPreG Σ} `{!crashPreG Σ} P `{!Plain P} ns n:
+  (∀ (Hi': invG Σ) Hc', NC 1-∗ |={⊤}=>
+   ∃ (pG: perennialG Λ CS T Σ) (Hpf: ∀ Hc t, @iris_invG _ _ (perennial_irisG Hc t) = Hi') t,
+     |={⊤}=> step_fupdN_fresh ns Hc' t
+                  (λ _ _, |={⊤}[∅]▷=>^(S n) |={⊤, ∅}_2=> P)) -∗
+  ▷^(fresh_later_count ns + S n) P.
+Proof.
+  iIntros "H".
+  iMod wsat_alloc' as (Hinv) "(Hw&HE)".
+  iSpecialize ("H" $! Hinv).
+  rewrite {1}uPred_fupd_eq {1}/uPred_fupd_def.
+  iApply (bupd_plain (▷^(_) P)%I); try (iPureIntro; apply _).
+  iMod NC_alloc as (Hc) "HNC".
+  rewrite {1}uPred_fupd_eq {1}/uPred_fupd_def.
+  iDestruct (ownE_weaken _ (AlwaysEn ∪ MaybeEn ⊤) with "HE") as "HE"; first by set_solver.
+  rewrite plus_comm. iEval (simpl).
+  iMod ("H" with "[$] [$]") as "[>Hw [>HE >H]]"; eauto.
+  iDestruct "H" as (pG Hpf t) "H".
+  iMod ("H" with "[$]") as "[>Hw [>HE >H]]"; eauto.
+
+  (* Have to strengthen the induction hypothesis to not lose wsat and ownE *)
+  iAssert (|={⊤}=> ▷ ▷^(n + fresh_later_count ns) P)%I with "[H]" as "Hgoal"; last first.
+  {
+    rewrite {1}uPred_fupd_eq {1}/uPred_fupd_def.
+    iMod ("Hgoal" with "[$]") as "[Hw [HE >H]]"; eauto.
+  }
+
+  iInduction ns as [| n' ns] "IH" forall (t Hc).
+  - rewrite /step_fupdN_fresh.
+    iDestruct (step_fupdN_fresh_pattern_plain' _ (P)%I with "H") as "H".
+    iMod ("H"). iModIntro. rewrite plus_comm. simpl. iFrame.
+  - iMod NC_alloc as (Hc') "HNC".
+    rewrite /step_fupdN_fresh -/step_fupdN_fresh.
+    iDestruct (step_fupdN_fresh_pattern_fupd _ _
+                  (▷^(S _ + fresh_later_count ns) P)%I
+                 with "H [IH HNC]") as "H".
+    { iIntros "H".
+      iSpecialize ("H" with "[$]").
+      rewrite ?Hpf.
+      iMod "H". iDestruct "H" as (t') "H".
+      by iApply ("IH").
+    }
+    iDestruct (step_fupdN_fresh_pattern_plain'' with "H") as "H".
+    rewrite ?Hpf.
+    iMod "H". iModIntro. rewrite plus_comm. simpl. iFrame.
+Qed.
+
+Lemma step_fupdN_fresh_soundness {Λ CS T Σ} `{!invPreG Σ} `{!crashPreG Σ} (φ : Prop) ns n:
+  (∀ (Hi: invG Σ) (Hc: crashG Σ), NC 1 ={⊤}=∗
+    ∃ (pG: perennialG Λ CS T Σ) (Hpf: ∀ Hc t, @iris_invG _ _ (perennial_irisG Hc t) = Hi) t0,
+      (|={⊤}=> step_fupdN_fresh ns Hc t0 (λ _ _, |={⊤}[∅]▷=>^((S (S n))) |={⊤, ∅}_2=> ⌜φ⌝))%I) →
+  φ.
+Proof.
+  intros Hiter.
+  eapply (soundness (M:=iResUR Σ) _  (fresh_later_count ns + _)); simpl.
+  rewrite laterN_plus.
+  iApply step_fupdN_fresh_plain. iIntros (Hinv Hc). iApply Hiter.
+Qed.
 
 Record recv_adequate {Λ CS} (s : stuckness) (e1 r1: expr Λ) (σ1 : state Λ)
     (φ φr: val Λ → state Λ → Prop) (φinv: state Λ → Prop)  := {
@@ -348,17 +390,17 @@ Qed.
 Corollary wp_recv_adequacy_inv Σ Λ CS (T: ofeT) `{!invPreG Σ} `{!crashPreG Σ} s k e r σ φ φr φinv Φinv :
   (∀ `{Hinv : !invG Σ} `{Hc: !crashG Σ} κs,
      ⊢ |={⊤}=> ∃ (t: pbundleG T Σ)
-         (stateI : invG Σ → pbundleG T Σ→ state Λ → list (observation Λ) → iProp Σ)
-         (fork_post : pbundleG T Σ → val Λ → iProp Σ) Hpf1 Hpf2,
+         (stateI : pbundleG T Σ→ state Λ → list (observation Λ) → iProp Σ)
+         (fork_post : pbundleG T Σ → val Λ → iProp Σ) Hpf1,
         let _ : perennialG Λ CS _ Σ :=
             PerennialG _ _ T Σ
-              (λ Hi Hc t,
-               IrisG Λ Σ Hi Hc (λ σ κs _, stateI Hi t σ κs)
-                    (fork_post t)) Hpf1 Hpf2
+              (λ Hc t,
+               IrisG Λ Σ Hinv Hc (λ σ κs _, stateI t σ κs)
+                    (fork_post t)) Hpf1
                in
-       □ (∀ σ κ, stateI Hinv t σ κ -∗ |NC={⊤, ∅}=> ⌜ φinv σ ⌝) ∗
-       □ (∀ Hi Hc t, Φinv Hi Hc t -∗ □ ∀ σ κ, stateI Hi t σ κ -∗ |NC={⊤, ∅}=> ⌜ φinv σ ⌝) ∗
-       stateI Hinv t σ κs ∗ wpr s k Hinv Hc t ⊤ e r (λ v, ⌜φ v⌝) Φinv (λ _ _ _ v, ⌜φr v⌝)) →
+       □ (∀ σ κ, stateI t σ κ -∗ |NC={⊤, ∅}=> ⌜ φinv σ ⌝) ∗
+       □ (∀ Hc t, Φinv Hinv Hc t -∗ □ ∀ σ κ, stateI t σ κ -∗ |NC={⊤, ∅}=> ⌜ φinv σ ⌝) ∗
+       stateI t σ κs ∗ wpr s k Hc t ⊤ e r (λ v, ⌜φ v⌝) (Φinv Hinv) (λ _ _ v, ⌜φr v⌝)) →
   recv_adequate (CS := CS) s e r σ (λ v _, φ v) (λ v _, φr v) φinv.
 Proof.
   intros Hwp.
@@ -367,18 +409,21 @@ Proof.
   destruct (nrsteps_snoc _ _ _ _ _ _ H) as (ns'&n'&->).
   eapply (step_fupdN_fresh_soundness _ ns' n')=> Hinv Hc.
   iIntros "HNC".
-  iMod (Hwp Hinv Hc κs) as (t stateI Hfork_post Hpf1 Hpf2) "(#Hinv1&#Hinv2&Hw&H)".
+  iMod (Hwp Hinv Hc κs) as (t stateI Hfork_post Hpf1) "(#Hinv1&#Hinv2&Hw&H)".
   iModIntro. iExists _.
   iDestruct (wptp_recv_strong_adequacy
                (perennialG0 :=
           PerennialG _ _ T Σ
-            (λ Hi Hc t,
-             IrisG Λ Σ Hi Hc (λ σ κs _, stateI Hi t σ κs)
-                  (Hfork_post t)) Hpf1 Hpf2) _ _ (λ Hi Hc t, (∀ σ κ, stateI Hi t σ κ -∗ |NC={⊤, ∅}=> ⌜ φinv σ ⌝))%I
+            (λ Hc t,
+             IrisG Λ Σ Hinv Hc (λ σ κs _, stateI t σ κs)
+                  (Hfork_post t)) Hpf1) _ _ (λ Hc t, (∀ σ κ, stateI t σ κ -∗ |NC={⊤, ∅}=> ⌜ φinv σ ⌝))%I
                _ [] with "[Hw] [H] [] [] HNC") as "H"; eauto.
   { rewrite app_nil_r. eauto. }
+  iExists _.
+  iExists t.
   iApply (step_fupdN_fresh_wand with "H").
-  iIntros (???) "H".
+  iModIntro.
+  iIntros (??) "H".
   iApply (step_fupdN_wand with "H"); auto.
   iIntros "H".
   iDestruct "H" as (v2 ???) "(Hw&Hv&Hnstuck&HNC)".
@@ -392,7 +437,7 @@ Proof.
     iIntros (v2' ? Heq). subst. inversion Heq; subst.
     rewrite to_of_val. naive_solver.
   - iDestruct "Hv" as "(Heq1&Hv)".
-    iDestruct "Heq1" as %(?&?&?); subst.
+    iDestruct "Heq1" as %(?&?); subst.
     rewrite ?ncfupd_eq /ncfupd_def.
     iMod ("Hinv1" with "[$] [$]") as "(Hp&HNC)".
     iDestruct "Hp" as %?.
@@ -400,4 +445,5 @@ Proof.
     iSplit; [| iSplit]; eauto.
     iIntros (v2' ? Heq). subst. inversion Heq; subst.
     rewrite to_of_val. naive_solver.
+  Unshelve. eauto.
 Qed.
