src/program_logic/recovery_weakestpre.v
@@ -14,35 +14,34 @@ Class pbundleG (T: ofeT) (Σ: gFunctors) := {
 }.
 
 Class perennialG (Λ : language) (CS: crash_semantics Λ) (T: ofeT) (Σ : gFunctors) := PerennialG {
-  perennial_irisG :> ∀ (H: invG Σ) (Hcrash: crashG Σ), pbundleG T Σ → irisG Λ Σ;
-  perennial_invG: ∀ H1 H2 t, @iris_invG _ _ (perennial_irisG H1 H2 t) = H1;
-  perennial_crashG: ∀ H1 H2 t, @iris_crashG _ _ (perennial_irisG H1 H2 t) = H2
+  perennial_irisG :> ∀ (Hcrash: crashG Σ), pbundleG T Σ → irisG Λ Σ;
+  perennial_crashG: ∀ H2 t, @iris_crashG _ _ (perennial_irisG H2 t) = H2
 }.
 
 Definition wpr_pre `{perennialG Λ CS T Σ} (s : stuckness) (k: nat)
-    (wpr : invG Σ -d> crashG Σ -d> pbundleG T Σ -d> coPset -d> expr Λ -d> expr Λ -d> (val Λ -d> iPropO Σ) -d>
-                     (invG Σ -d> crashG Σ -d> pbundleG T Σ -d> iPropO Σ) -d>
-                     (invG Σ -d> crashG Σ -d> pbundleG T Σ -d> val Λ -d> iPropO Σ) -d> iPropO Σ) :
-  invG Σ -d> crashG Σ -d> pbundleG T Σ -d> coPset -d> expr Λ -d> expr Λ -d> (val Λ -d> iPropO Σ) -d>
-  (invG Σ -d> crashG Σ -d> pbundleG T Σ -d> iPropO Σ) -d>
-  (invG Σ -d> crashG Σ -d> pbundleG T Σ -d> val Λ -d> iPropO Σ) -d> iPropO Σ :=
-  λ H1 H2 t E e rec Φ Φinv Φr,
+    (wpr : crashG Σ -d> pbundleG T Σ -d> coPset -d> expr Λ -d> expr Λ -d> (val Λ -d> iPropO Σ) -d>
+                     (crashG Σ -d> pbundleG T Σ -d> iPropO Σ) -d>
+                     (crashG Σ -d> pbundleG T Σ -d> val Λ -d> iPropO Σ) -d> iPropO Σ) :
+  crashG Σ -d> pbundleG T Σ -d> coPset -d> expr Λ -d> expr Λ -d> (val Λ -d> iPropO Σ) -d>
+  (crashG Σ -d> pbundleG T Σ -d> iPropO Σ) -d>
+  (crashG Σ -d> pbundleG T Σ -d> val Λ -d> iPropO Σ) -d> iPropO Σ :=
+  λ H2 t E e rec Φ Φinv Φr,
   (WPC e @ s ; k; E
      {{ Φ }}
      {{ ∀ σ σ' (HC: crash_prim_step CS σ σ') κs n,
-        state_interp σ κs n ={∅}=∗  ▷ ∀ H1 H2 q, NC q ={⊤}=∗ ∃ t, state_interp σ' κs 0 ∗ (Φinv H1 H2 t ∧ wpr H1 H2 t E rec rec (λ v, Φr H1 H2 t v) Φinv Φr) ∗ NC q}})%I.
+        state_interp σ κs n ={E}=∗  ▷ ∀ H2 q, NC q ={E}=∗ ∃ t, state_interp σ' κs 0 ∗ (Φinv H2 t ∧ wpr H2 t E rec rec (λ v, Φr H2 t v) Φinv Φr) ∗ NC q}})%I.
 
 Local Instance wpr_pre_contractive `{!perennialG Λ CS T Σ} s k: Contractive (wpr_pre s k).
 Proof.
-  rewrite /wpr_pre=> n wp wp' Hwp H1inv H2crash t E1 e1 rec Φ Φinv Φc.
+  rewrite /wpr_pre=> n wp wp' Hwp H2crash t E1 e1 rec Φ Φinv Φc.
   apply wpc_ne; eauto;
   repeat (f_contractive || f_equiv). apply Hwp.
 Qed.
 
 Definition wpr_def `{!perennialG Λ CS T Σ} (s : stuckness) k :
-  invG Σ → crashG Σ → pbundleG T Σ → coPset → expr Λ → expr Λ → (val Λ → iProp Σ) →
-  (invG Σ → crashG Σ → pbundleG T Σ → iProp Σ) →
-  (invG Σ → crashG Σ → pbundleG T Σ → val Λ → iProp Σ) → iProp Σ := fixpoint (wpr_pre s k).
+  crashG Σ → pbundleG T Σ → coPset → expr Λ → expr Λ → (val Λ → iProp Σ) →
+  (crashG Σ → pbundleG T Σ → iProp Σ) →
+  (crashG Σ → pbundleG T Σ → val Λ → iProp Σ) → iProp Σ := fixpoint (wpr_pre s k).
 Definition wpr_aux `{!perennialG Λ CS T Σ} : seal (@wpr_def Λ CS T Σ _). by eexists. Qed.
 Definition wpr `{!perennialG Λ CS T Σ} := wpr_aux.(unseal).
 Definition wpr_eq `{!perennialG Λ CS T Σ} : wpr = @wpr_def Λ CS T Σ _ := wpr_aux.(seal_eq).
@@ -53,22 +52,22 @@ Implicit Types s : stuckness.
 Implicit Types k : nat.
 Implicit Types P : iProp Σ.
 Implicit Types Φ : val Λ → iProp Σ.
-Implicit Types Φc : invG Σ → crashG Σ → pbundleG T Σ → val Λ → iProp Σ.
+Implicit Types Φc : crashG Σ → pbundleG T Σ → val Λ → iProp Σ.
 Implicit Types v : val Λ.
 Implicit Types e : expr Λ.
 
-Lemma wpr_unfold s k Hi Hc t E e rec Φ Φinv Φc :
-  wpr s k Hi Hc t E e rec Φ Φinv Φc ⊣⊢ wpr_pre s k (wpr s k) Hi Hc t E e rec Φ Φinv Φc.
+Lemma wpr_unfold s k Hc t E e rec Φ Φinv Φc :
+  wpr s k Hc t E e rec Φ Φinv Φc ⊣⊢ wpr_pre s k (wpr s k) Hc t E e rec Φ Φinv Φc.
 Proof. rewrite wpr_eq. apply (fixpoint_unfold (wpr_pre s k)). Qed.
 
 (* There's a stronger version of this *)
-Lemma wpr_strong_mono s k Hi Hc t E e rec Φ Ψ Φinv Ψinv Φr Ψr :
-  wpr s k Hi Hc t E e rec Φ Φinv Φr -∗
-      (∀ v, Φ v ==∗ Ψ v) ∧ <bdisc> ((∀ Hi Hc t, Φinv Hi Hc t -∗ Ψinv Hi Hc t) ∧
-                                    (∀ Hi Hc t v, Φr Hi Hc t v ==∗ Ψr Hi Hc t v)) -∗
-  wpr s k Hi Hc t E e rec Ψ Ψinv Ψr.
+Lemma wpr_strong_mono s k Hc t E e rec Φ Ψ Φinv Ψinv Φr Ψr :
+  wpr s k Hc t E e rec Φ Φinv Φr -∗
+      (∀ v, Φ v ==∗ Ψ v) ∧ <bdisc> ((∀ Hc t, Φinv Hc t -∗ Ψinv Hc t) ∧
+                                    (∀ Hc t v, Φr Hc t v ==∗ Ψr Hc t v)) -∗
+  wpr s k Hc t E e rec Ψ Ψinv Ψr.
 Proof.
-  iIntros "H HΦ". iLöb as "IH" forall (e t Hi Hc E Φ Ψ Φinv Ψinv Φr Ψr).
+  iIntros "H HΦ". iLöb as "IH" forall (e t Hc E Φ Ψ Φinv Ψinv Φr Ψr).
   rewrite ?wpr_unfold /wpr_pre.
   iApply (wpc_strong_mono' with "H") ; auto.
   iSplit.
@@ -77,7 +76,7 @@ Proof.
   rewrite own_discrete_idemp.
   iIntros "!> H".
   iModIntro. iIntros (?????) "Hinterp". iMod ("H" with "[//] Hinterp") as "H".
-  iModIntro. iNext. iIntros (Hi' Hc' ?) "HNC". iMod ("H" $! Hi' Hc' with "[$]") as (?) "(?&H&HNC)".
+  iModIntro. iNext. iIntros (Hc' ?) "HNC". iMod ("H" $! Hc' with "[$]") as (?) "(?&H&HNC)".
   iModIntro. iExists _. iFrame.
   iSplit.
   - iDestruct "H" as "(H&_)". rewrite own_discrete_elim. iDestruct "HΦ" as "(HΦ&_)". by iApply "HΦ".
@@ -89,14 +88,14 @@ Qed.
 
 (* To prove a recovery wp for e with rec, it suffices to prove a crash wp for e,
    where the crash condition implies the precondition for a crash wp for rec *)
-Lemma idempotence_wpr s k E1 e rec Φx Φinv Φrx (Φcx: invG Σ → crashG Σ → _ → iProp Σ) Hi Hc t:
-  ⊢ WPC e @ s ; k ; E1 {{ Φx t }} {{ Φcx Hi _ t }} -∗
-   (□ ∀ (H: invG Σ) (Hc: crashG Σ) (t: pbundleG T Σ) σ σ' (HC: crash_prim_step CS σ σ') κs n,
-        Φcx H Hc t -∗ state_interp σ κs n ={∅}=∗
-        ▷ ∀ H' (Hc': crashG Σ) q, NC q ={⊤}=∗ ∃ t', state_interp σ' κs 0 ∗ (Φinv H' Hc' t' ∧ WPC rec @ s ; k; E1 {{ Φrx H' Hc' t' }} {{ Φcx H' Hc' t' }}) ∗ NC q) -∗
-    wpr s k Hi Hc t E1 e rec (Φx t) Φinv Φrx.
+Lemma idempotence_wpr s k E1 e rec Φx Φinv Φrx (Φcx: crashG Σ → _ → iProp Σ) Hc t:
+  ⊢ WPC e @ s ; k ; E1 {{ Φx t }} {{ Φcx _ t }} -∗
+   (□ ∀ (Hc: crashG Σ) (t: pbundleG T Σ) σ σ' (HC: crash_prim_step CS σ σ') κs n,
+        Φcx Hc t -∗ state_interp σ κs n ={E1}=∗
+        ▷ ∀ (Hc': crashG Σ) q, NC q ={E1}=∗ ∃ t', state_interp σ' κs 0 ∗ (Φinv Hc' t' ∧ WPC rec @ s ; k; E1 {{ Φrx Hc' t' }} {{ Φcx Hc' t' }}) ∗ NC q) -∗
+    wpr s k Hc t E1 e rec (Φx t) Φinv Φrx.
 Proof.
-  iLöb as "IH" forall (E1 e Hi Hc t Φx).
+  iLöb as "IH" forall (E1 e Hc t Φx).
   iIntros  "He #Hidemp".
   rewrite wpr_unfold. rewrite /wpr_pre.
   iApply (wpc_strong_mono' with "He"); [ auto | auto | auto | ].
@@ -105,12 +104,12 @@ Proof.
   { set_solver +. }
   iIntros. iMod ("Hidemp" with "[ ] [$] [$]") as "H".
   { eauto. }
-  iModIntro. iNext. iIntros (Hi' Hc' ?) "HNC". iMod ("H" $! Hi' Hc' with "[$]") as (t') "(?&Hc&HNC)".
+  iModIntro. iNext. iIntros (Hc' ?) "HNC". iMod ("H" $! Hc' with "[$]") as (t') "(?&Hc&HNC)".
   iExists _. iFrame. iModIntro.
   iSplit.
   { iDestruct "Hc" as "($&_)". }
   iDestruct "Hc" as "(_&Hc)".
-  iApply ("IH" $! E1 rec Hi' Hc' t' (λ t v, Φrx Hi' Hc' t v)%I with " [Hc]").
+  iApply ("IH" $! E1 rec Hc' t' (λ t v, Φrx Hc' t v)%I with " [Hc]").
   { iApply (wpc_strong_mono' with "Hc"); auto. }
   eauto.
 Qed.
